% Emacs, this is -*- latex -*-!
\begin{figure}
\begin{align*}
\Derive{\Lit n}
& = \Lit0\\
\Derive{\Add{t_1}{t_2}}
& = \Add{\Derive{t_1}}{\Derive{t_2}}\\
\Derive{\Minus t}
& = \Minus{\Derive t}\\
\Derive{\Singleton{n_1,\ldots,n_m}}
& = \Singleton{}\\
\Derive{\Union{t_1}{t_2}}
& = \Union{\Derive{t_1}}{\Derive{t_2}}\\
\Derive{\Negate t}
& = \Negate{\Derive t}\\
\Derive{\Map{t_1}{t_2}}
& = {\Map*{\Apply*{\Derive{t_1}}{t_1}}
          {\Apply*{\Derive{t_2}}{t_2}}}\\
&\,\DIFF\, {\Map*{t_1}{t_2}}\\
\Derive{\Sum t}
& = {\Sum{\Derive t}}
\end{align*}
\caption{Derivation.}\pg{reference the function part in the appendix~\ref{sec:STLC-correct}. }
\label{fig:plug-derive}
\end{figure}
